---
title: The distance between natural numbers
---

```agda
{-# OPTIONS --without-K --exact-split #-}

module elementary-number-theory.distance-natural-numbers where

open import elementary-number-theory.addition-natural-numbers using
  ( add-ℕ; add-ℕ'; ap-add-ℕ; left-unit-law-add-ℕ; left-successor-law-add-ℕ;
    commutative-add-ℕ)
open import elementary-number-theory.inequality-natural-numbers using
  ( leq-ℕ; _≤-ℕ_; refl-leq-ℕ; concatenate-eq-leq-eq-ℕ; concatenate-leq-eq-ℕ;
    transitive-leq-ℕ; succ-leq-ℕ; order-three-elements-ℕ; le-ℕ;
    preserves-le-succ-ℕ)
open import elementary-number-theory.multiplication-natural-numbers using
  ( mul-ℕ; right-zero-law-mul-ℕ; right-successor-law-mul-ℕ; commutative-mul-ℕ)
open import elementary-number-theory.natural-numbers using
  ( ℕ; zero-ℕ; succ-ℕ; is-zero-ℕ; is-one-ℕ)
  
open import foundation.coproduct-types using (_+_; inl; inr)
open import foundation.dependent-pair-types using (pair)
open import foundation.functions using (_∘_)
open import foundation.identity-types using
  ( _＝_; refl; _∙_; inv; ap; ap-binary; tr)
open import foundation.unit-type using (star)
open import foundation.universe-levels using (UU; lzero)
```

## Definition

```agda
-- We define a distance function on ℕ --

dist-ℕ : ℕ → ℕ → ℕ
dist-ℕ zero-ℕ n = n
dist-ℕ (succ-ℕ m) zero-ℕ = succ-ℕ m
dist-ℕ (succ-ℕ m) (succ-ℕ n) = dist-ℕ m n

dist-ℕ' : ℕ → ℕ → ℕ
dist-ℕ' m n = dist-ℕ n m

ap-dist-ℕ :
  {m n m' n' : ℕ} → m ＝ m' → n ＝ n' → dist-ℕ m n ＝ dist-ℕ m' n'
ap-dist-ℕ p q = ap-binary dist-ℕ p q

{- We show that two natural numbers are equal if and only if their distance is
   zero. -}

eq-dist-ℕ : (m n : ℕ) → is-zero-ℕ (dist-ℕ m n) → m ＝ n
eq-dist-ℕ zero-ℕ zero-ℕ p = refl
eq-dist-ℕ (succ-ℕ m) (succ-ℕ n) p = ap succ-ℕ (eq-dist-ℕ m n p)

dist-eq-ℕ' : (n : ℕ) → is-zero-ℕ (dist-ℕ n n)
dist-eq-ℕ' zero-ℕ = refl
dist-eq-ℕ' (succ-ℕ n) = dist-eq-ℕ' n

dist-eq-ℕ : (m n : ℕ) → m ＝ n → is-zero-ℕ (dist-ℕ m n)
dist-eq-ℕ m .m refl = dist-eq-ℕ' m

is-one-dist-succ-ℕ : (x : ℕ) → is-one-ℕ (dist-ℕ x (succ-ℕ x))
is-one-dist-succ-ℕ zero-ℕ = refl
is-one-dist-succ-ℕ (succ-ℕ x) = is-one-dist-succ-ℕ x

is-one-dist-succ-ℕ' : (x : ℕ) → is-one-ℕ (dist-ℕ (succ-ℕ x) x)
is-one-dist-succ-ℕ' zero-ℕ = refl
is-one-dist-succ-ℕ' (succ-ℕ x) = is-one-dist-succ-ℕ' x

-- The distance function is symmetric --

symmetric-dist-ℕ :
  (m n : ℕ) → dist-ℕ m n ＝ dist-ℕ n m
symmetric-dist-ℕ zero-ℕ zero-ℕ = refl
symmetric-dist-ℕ zero-ℕ (succ-ℕ n) = refl
symmetric-dist-ℕ (succ-ℕ m) zero-ℕ = refl
symmetric-dist-ℕ (succ-ℕ m) (succ-ℕ n) = symmetric-dist-ℕ m n

-- We compute the distance from zero --

left-unit-law-dist-ℕ :
  (n : ℕ) → dist-ℕ zero-ℕ n ＝ n
left-unit-law-dist-ℕ zero-ℕ = refl
left-unit-law-dist-ℕ (succ-ℕ n) = refl

right-unit-law-dist-ℕ :
  (n : ℕ) → dist-ℕ n zero-ℕ ＝ n
right-unit-law-dist-ℕ zero-ℕ = refl
right-unit-law-dist-ℕ (succ-ℕ n) = refl

-- We prove the triangle inequality --

triangle-inequality-dist-ℕ :
  (m n k : ℕ) → (dist-ℕ m n) ≤-ℕ (add-ℕ (dist-ℕ m k) (dist-ℕ k n))
triangle-inequality-dist-ℕ zero-ℕ zero-ℕ zero-ℕ = star
triangle-inequality-dist-ℕ zero-ℕ zero-ℕ (succ-ℕ k) = star
triangle-inequality-dist-ℕ zero-ℕ (succ-ℕ n) zero-ℕ =
  tr ( leq-ℕ (succ-ℕ n))
     ( inv (left-unit-law-add-ℕ (succ-ℕ n)))
     ( refl-leq-ℕ (succ-ℕ n))
triangle-inequality-dist-ℕ zero-ℕ (succ-ℕ n) (succ-ℕ k) =
  concatenate-eq-leq-eq-ℕ
    ( inv (ap succ-ℕ (left-unit-law-dist-ℕ n)))
    ( triangle-inequality-dist-ℕ zero-ℕ n k)
    ( ( ap (succ-ℕ ∘ (add-ℕ' (dist-ℕ k n))) (left-unit-law-dist-ℕ k)) ∙
      ( inv (left-successor-law-add-ℕ k (dist-ℕ k n))))
triangle-inequality-dist-ℕ (succ-ℕ m) zero-ℕ zero-ℕ = refl-leq-ℕ (succ-ℕ m)
triangle-inequality-dist-ℕ (succ-ℕ m) zero-ℕ (succ-ℕ k) =
  concatenate-eq-leq-eq-ℕ
    ( inv (ap succ-ℕ (right-unit-law-dist-ℕ m)))
    ( triangle-inequality-dist-ℕ m zero-ℕ k)
    ( ap (succ-ℕ ∘ (add-ℕ (dist-ℕ m k))) (right-unit-law-dist-ℕ k))
triangle-inequality-dist-ℕ (succ-ℕ m) (succ-ℕ n) zero-ℕ =
  concatenate-leq-eq-ℕ
    ( dist-ℕ m n)
    ( transitive-leq-ℕ
      ( dist-ℕ m n)
      ( succ-ℕ (add-ℕ (dist-ℕ m zero-ℕ) (dist-ℕ zero-ℕ n)))
      ( succ-ℕ (succ-ℕ (add-ℕ (dist-ℕ m zero-ℕ) (dist-ℕ zero-ℕ n))))
      ( succ-leq-ℕ (succ-ℕ (add-ℕ (dist-ℕ m zero-ℕ) (dist-ℕ zero-ℕ n))))
      ( transitive-leq-ℕ
        ( dist-ℕ m n)
        ( add-ℕ (dist-ℕ m zero-ℕ) (dist-ℕ zero-ℕ n))
        ( succ-ℕ (add-ℕ (dist-ℕ m zero-ℕ) (dist-ℕ zero-ℕ n)))
        ( succ-leq-ℕ (add-ℕ (dist-ℕ m zero-ℕ) (dist-ℕ zero-ℕ n)))
        ( triangle-inequality-dist-ℕ m n zero-ℕ)))
    ( ( ap (succ-ℕ ∘ succ-ℕ)
           ( ap-add-ℕ (right-unit-law-dist-ℕ m) (left-unit-law-dist-ℕ n))) ∙
      ( inv (left-successor-law-add-ℕ m (succ-ℕ n))))

triangle-inequality-dist-ℕ (succ-ℕ m) (succ-ℕ n) (succ-ℕ k) =
  triangle-inequality-dist-ℕ m n k

-- Exercise 6.5 (b)

-- We show that dist-ℕ x y is a solution to a simple equation.

is-additive-right-inverse-dist-ℕ :
  (x y : ℕ) → x ≤-ℕ y → add-ℕ x (dist-ℕ x y) ＝ y
is-additive-right-inverse-dist-ℕ zero-ℕ zero-ℕ H = refl
is-additive-right-inverse-dist-ℕ zero-ℕ (succ-ℕ y) star = left-unit-law-add-ℕ (succ-ℕ y)
is-additive-right-inverse-dist-ℕ (succ-ℕ x) (succ-ℕ y) H =
  ( left-successor-law-add-ℕ x (dist-ℕ x y)) ∙
  ( ap succ-ℕ (is-additive-right-inverse-dist-ℕ x y H))

-- If three elements are ordered linearly, then their distances add up.

triangle-equality-dist-ℕ :
  (x y z : ℕ) → (x ≤-ℕ y) → (y ≤-ℕ z) →
  add-ℕ (dist-ℕ x y) (dist-ℕ y z) ＝ dist-ℕ x z
triangle-equality-dist-ℕ zero-ℕ zero-ℕ zero-ℕ H1 H2 = refl
triangle-equality-dist-ℕ zero-ℕ zero-ℕ (succ-ℕ z) star star =
  ap succ-ℕ (left-unit-law-add-ℕ z)
triangle-equality-dist-ℕ zero-ℕ (succ-ℕ y) (succ-ℕ z) star H2 =
  left-successor-law-add-ℕ y (dist-ℕ y z) ∙
  ap succ-ℕ (is-additive-right-inverse-dist-ℕ y z H2)
triangle-equality-dist-ℕ (succ-ℕ x) (succ-ℕ y) (succ-ℕ z) H1 H2 =
  triangle-equality-dist-ℕ x y z H1 H2

rewrite-left-add-dist-ℕ :
  (x y z : ℕ) → add-ℕ x y ＝ z → x ＝ dist-ℕ y z
rewrite-left-add-dist-ℕ zero-ℕ zero-ℕ .zero-ℕ refl = refl
rewrite-left-add-dist-ℕ zero-ℕ (succ-ℕ y) .(succ-ℕ (add-ℕ zero-ℕ y)) refl =
  ( inv (dist-eq-ℕ' y)) ∙
  ( inv (ap (dist-ℕ (succ-ℕ y)) (left-unit-law-add-ℕ (succ-ℕ y))))
rewrite-left-add-dist-ℕ (succ-ℕ x) zero-ℕ .(succ-ℕ x) refl = refl
rewrite-left-add-dist-ℕ
  (succ-ℕ x) (succ-ℕ y) .(succ-ℕ (add-ℕ (succ-ℕ x) y)) refl =
  rewrite-left-add-dist-ℕ (succ-ℕ x) y (add-ℕ (succ-ℕ x) y) refl

rewrite-left-dist-add-ℕ :
  (x y z : ℕ) → y ≤-ℕ z → x ＝ dist-ℕ y z → add-ℕ x y ＝ z
rewrite-left-dist-add-ℕ .(dist-ℕ y z) y z H refl =
  ( commutative-add-ℕ (dist-ℕ y z) y) ∙
  ( is-additive-right-inverse-dist-ℕ y z H)

rewrite-right-add-dist-ℕ :
  (x y z : ℕ) → add-ℕ x y ＝ z → y ＝ dist-ℕ x z
rewrite-right-add-dist-ℕ x y z p =
  rewrite-left-add-dist-ℕ y x z (commutative-add-ℕ y x ∙ p)

rewrite-right-dist-add-ℕ :
  (x y z : ℕ) → x ≤-ℕ z → y ＝ dist-ℕ x z → add-ℕ x y ＝ z
rewrite-right-dist-add-ℕ x .(dist-ℕ x z) z H refl =
  is-additive-right-inverse-dist-ℕ x z H

leq-dist-ℕ :
  (x y : ℕ) → x ≤-ℕ y → dist-ℕ x y ≤-ℕ y
leq-dist-ℕ zero-ℕ zero-ℕ H = refl-leq-ℕ zero-ℕ
leq-dist-ℕ zero-ℕ (succ-ℕ y) H = refl-leq-ℕ y
leq-dist-ℕ (succ-ℕ x) (succ-ℕ y) H =
  transitive-leq-ℕ (dist-ℕ x y) y (succ-ℕ y) (succ-leq-ℕ y) (leq-dist-ℕ x y H)

-- We show that dist-ℕ is translation invariant

translation-invariant-dist-ℕ :
  (k m n : ℕ) → dist-ℕ (add-ℕ k m) (add-ℕ k n) ＝ dist-ℕ m n
translation-invariant-dist-ℕ zero-ℕ m n =
  ap-dist-ℕ (left-unit-law-add-ℕ m) (left-unit-law-add-ℕ n)
translation-invariant-dist-ℕ (succ-ℕ k) m n =
  ( ap-dist-ℕ (left-successor-law-add-ℕ k m) (left-successor-law-add-ℕ k n)) ∙
  ( translation-invariant-dist-ℕ k m n)

translation-invariant-dist-ℕ' :
  (k m n : ℕ) → dist-ℕ (add-ℕ m k) (add-ℕ n k) ＝ dist-ℕ m n
translation-invariant-dist-ℕ' k m n =
  ( ap-dist-ℕ (commutative-add-ℕ m k) (commutative-add-ℕ n k)) ∙
  ( translation-invariant-dist-ℕ k m n)

-- We show that dist-ℕ is linear with respect to scalar multiplication

left-distributive-mul-dist-ℕ :
  (m n k : ℕ) → mul-ℕ k (dist-ℕ m n) ＝ dist-ℕ (mul-ℕ k m) (mul-ℕ k n)
left-distributive-mul-dist-ℕ zero-ℕ zero-ℕ zero-ℕ = refl
left-distributive-mul-dist-ℕ zero-ℕ zero-ℕ (succ-ℕ k) = left-distributive-mul-dist-ℕ zero-ℕ zero-ℕ k
left-distributive-mul-dist-ℕ zero-ℕ (succ-ℕ n) zero-ℕ = refl
left-distributive-mul-dist-ℕ zero-ℕ (succ-ℕ n) (succ-ℕ k) =
  ap ( dist-ℕ' (mul-ℕ (succ-ℕ k) (succ-ℕ n)))
     ( inv (right-zero-law-mul-ℕ (succ-ℕ k)))
left-distributive-mul-dist-ℕ (succ-ℕ m) zero-ℕ zero-ℕ = refl
left-distributive-mul-dist-ℕ (succ-ℕ m) zero-ℕ (succ-ℕ k) =
  ap ( dist-ℕ (mul-ℕ (succ-ℕ k) (succ-ℕ m)))
     ( inv (right-zero-law-mul-ℕ (succ-ℕ k)))
left-distributive-mul-dist-ℕ (succ-ℕ m) (succ-ℕ n) zero-ℕ = refl
left-distributive-mul-dist-ℕ (succ-ℕ m) (succ-ℕ n) (succ-ℕ k) =
  inv
    ( ( ap-dist-ℕ
        ( right-successor-law-mul-ℕ (succ-ℕ k) m)
        ( right-successor-law-mul-ℕ (succ-ℕ k) n)) ∙
      ( ( translation-invariant-dist-ℕ
          ( succ-ℕ k)
          ( mul-ℕ (succ-ℕ k) m)
          ( mul-ℕ (succ-ℕ k) n)) ∙
        ( inv (left-distributive-mul-dist-ℕ m n (succ-ℕ k)))))

right-distributive-mul-dist-ℕ :
  (x y k : ℕ) → mul-ℕ (dist-ℕ x y) k ＝ dist-ℕ (mul-ℕ x k) (mul-ℕ y k)
right-distributive-mul-dist-ℕ x y k =
  ( commutative-mul-ℕ (dist-ℕ x y) k) ∙
  ( ( left-distributive-mul-dist-ℕ x y k) ∙
    ( ap-dist-ℕ (commutative-mul-ℕ k x) (commutative-mul-ℕ k y)))

-- Exercise 6.5 (d)

is-difference-dist-ℕ :
  (x y : ℕ) → x ≤-ℕ y → add-ℕ x (dist-ℕ x y) ＝ y
is-difference-dist-ℕ zero-ℕ zero-ℕ H = refl
is-difference-dist-ℕ zero-ℕ (succ-ℕ y) H = left-unit-law-add-ℕ (succ-ℕ y)
is-difference-dist-ℕ (succ-ℕ x) (succ-ℕ y) H =
  ( left-successor-law-add-ℕ x (dist-ℕ x y)) ∙
  ( ap succ-ℕ (is-difference-dist-ℕ x y H))

is-difference-dist-ℕ' :
  (x y : ℕ) → x ≤-ℕ y → add-ℕ (dist-ℕ x y) x ＝ y
is-difference-dist-ℕ' x y H =
  ( commutative-add-ℕ (dist-ℕ x y) x) ∙
  ( is-difference-dist-ℕ x y H)
```

```agda
cases-dist-ℕ :
  (x y z : ℕ) → UU lzero
cases-dist-ℕ x y z =
  ( add-ℕ (dist-ℕ x y) (dist-ℕ y z) ＝ dist-ℕ x z) +
  ( ( add-ℕ (dist-ℕ y z) (dist-ℕ x z) ＝ dist-ℕ x y) +
    ( add-ℕ (dist-ℕ x z) (dist-ℕ x y) ＝ dist-ℕ y z))

is-total-dist-ℕ :
  (x y z : ℕ) → cases-dist-ℕ x y z
is-total-dist-ℕ x y z with order-three-elements-ℕ x y z
is-total-dist-ℕ x y z | inl (inl (pair H1 H2)) =
  inl (triangle-equality-dist-ℕ x y z H1 H2)
is-total-dist-ℕ x y z | inl (inr (pair H1 H2)) =
  inr
    ( inl
      ( ( commutative-add-ℕ (dist-ℕ y z) (dist-ℕ x z)) ∙
        ( ( ap (add-ℕ (dist-ℕ x z)) (symmetric-dist-ℕ y z)) ∙
          ( triangle-equality-dist-ℕ x z y H1 H2))))
is-total-dist-ℕ x y z | inr (inl (inl (pair H1 H2))) =
  inr
    ( inl
      ( ( ap (add-ℕ (dist-ℕ y z)) (symmetric-dist-ℕ x z)) ∙
        ( ( triangle-equality-dist-ℕ y z x H1 H2) ∙
          ( symmetric-dist-ℕ y x))))
is-total-dist-ℕ x y z | inr (inl (inr (pair H1 H2))) =
  inr
    ( inr
      ( ( ap (add-ℕ (dist-ℕ x z)) (symmetric-dist-ℕ x y)) ∙
        ( ( commutative-add-ℕ (dist-ℕ x z) (dist-ℕ y x)) ∙
          ( triangle-equality-dist-ℕ y x z H1 H2))))
is-total-dist-ℕ x y z | inr (inr (inl (pair H1 H2))) =
  inr
    ( inr
      ( ( ap (add-ℕ' (dist-ℕ x y)) (symmetric-dist-ℕ x z)) ∙
        ( ( triangle-equality-dist-ℕ z x y H1 H2) ∙
          ( symmetric-dist-ℕ z y))))
is-total-dist-ℕ x y z | inr (inr (inr (pair H1 H2))) =
  inl
    ( ( ap-add-ℕ (symmetric-dist-ℕ x y) (symmetric-dist-ℕ y z)) ∙
      ( ( commutative-add-ℕ (dist-ℕ y x) (dist-ℕ z y)) ∙
        ( ( triangle-equality-dist-ℕ z y x H1 H2) ∙
          ( symmetric-dist-ℕ z x))))
```

```agda
strict-upper-bound-dist-ℕ :
  (b x y : ℕ) → le-ℕ x b → le-ℕ y b → le-ℕ (dist-ℕ x y) b
strict-upper-bound-dist-ℕ (succ-ℕ b) zero-ℕ y H K = K
strict-upper-bound-dist-ℕ (succ-ℕ b) (succ-ℕ x) zero-ℕ H K = H
strict-upper-bound-dist-ℕ (succ-ℕ b) (succ-ℕ x) (succ-ℕ y) H K =
  preserves-le-succ-ℕ (dist-ℕ x y) b (strict-upper-bound-dist-ℕ b x y H K)
```
